end of day 22/06/19

theories/SAL-examples/Byzantine_Drinks_Machine.thy
@@ -1,21 +1,6 @@
-section{*Examples*}
-subsection{*Drinks Machine*}
-text{*This theory formalises a simple drinks machine. The \emph{select} operation takes one
-argument - the desired beverage. The \emph{coin} operation also takes one parameter representing
-the value of the coin. The \emph{vend} operation has two flavours - one which dispenses the drink if
-the customer has inserted enough money, and one which dispenses nothing if the user has not inserted
-sufficient funds.
-
-We first define a datatype \emph{statemane} which corresponds to $S$ in the formal definition.
-Note that, while statename has four elements, the drinks machine presented here only requires three
-states. The fourth element is included here so that the \emph{statename} datatype may be used in
-the next example.
-*}
 theory Byzantine_Drinks_Machine
   imports "../Contexts"
 begin
-
-declare One_nat_def [simp del]
 
 definition select :: "transition" where
 "select \<equiv> \<lparr>
@@ -24,8 +9,8 @@ definition select :: "transition" where
         Guard = [], \<comment> \<open> No guards \<close>
         Outputs = [],
         Updates = [ \<comment> \<open> Two updates: \<close>
-                    (R 1, (V (I 1))), \<comment> \<open>  Firstly set value of r1 to value of i1 \<close>
-                    (R 2, (L (Num 0))) \<comment> \<open> Secondly set the value of r2 to literal zero \<close>
+                    (1, (V (I 1))), \<comment> \<open>  Firstly set value of r1 to value of i1 \<close>
+                    (2, (L (Num 0))) \<comment> \<open> Secondly set the value of r2 to literal zero \<close>
                   ]
       \<rparr>"
 
@@ -44,8 +29,8 @@ definition coin :: "transition" where
         Guard = [],
         Outputs = [Plus (V (R 2)) (V (I 1))],
         Updates = [
-                    (R 1, V (R 1)),
-                    (R 2, Plus (V (R 2)) (V (I 1)))
+                    (1, V (R 1)),
+                    (2, Plus (V (R 2)) (V (I 1)))
                   ]
       \<rparr>"
 
@@ -61,7 +46,7 @@ definition vend :: "transition" where
         Arity = 0,
         Guard = [(Ge (V (R 2)) (L (Num 100)))],
         Outputs =  [(V (R 1))],
-        Updates = [(R 1, V (R 1)), (R 2, V (R 2))]
+        Updates = [(1, V (R 1)), (2, V (R 2))]
       \<rparr>"
 
 lemma label_vend: "Label vend = STR ''vend''"
@@ -73,7 +58,7 @@ definition vend_fail :: "transition" where
         Arity = 0,
         Guard = [(GExp.Lt (V (R 2)) (L (Num 100)))],
         Outputs =  [],
-        Updates = [(R 1, V (R 1)), (R 2, V (R 2))]
+        Updates = [(1, V (R 1)), (2, V (R 2))]
       \<rparr>"
 
 definition drinks :: "transition_matrix" where
