theories/SAL-examples/Coin_Choc_Broken.thy
@@ -1,5 +1,5 @@
 theory Coin_Choc_Broken
-  imports EFSM_LTL
+  imports "../EFSM_LTL"
 begin
 
 declare One_nat_def [simp del]
@@ -11,7 +11,7 @@ definition init :: transition where
         Arity = 0,
         Guard = [],
         Outputs = [],
-        Updates = [(R 1, (L (Num 0)))]
+        Updates = [(1, (L (Num 0)))]
       \<rparr>"
 
 definition coin :: transition where
@@ -20,7 +20,7 @@ definition coin :: transition where
         Arity = 0,
         Guard = [],
         Outputs = [],
-        Updates = [(R 1, (Plus (V (R 1)) (L (Num 1))))]
+        Updates = [(1, (Plus (V (R 1)) (L (Num 1))))]
       \<rparr>"
 
 definition vend :: transition where
@@ -29,7 +29,7 @@ definition vend :: transition where
         Arity = 0,
         Guard = [GExp.Ge (V (R 1)) (L (Num 0))],
         Outputs = [],
-        Updates = [(R 1, (Minus (V (R 1)) (L (Num 1))))]
+        Updates = [(1, (Minus (V (R 1)) (L (Num 1))))]
       \<rparr>"
 
 definition drinks :: "transition_matrix" where
@@ -38,9 +38,6 @@ definition drinks :: "transition_matrix" where
           ((1,1), coin),
           ((1,2), vend)
           |}"
-
-lemma "(not (LabelEq ''vend'') until (LabelEq ''coin'')) (watch drinks t)"
-  oops
 
 lemma possible_steps_init: "possible_steps drinks 0 Map.empty STR ''init'' [] = {|(1, init)|}"
     apply (simp add: possible_steps_alt Abs_ffilter Set.filter_def drinks_def)
@@ -72,9 +69,9 @@ lemma make_full_obs_neq: "make_full_observation drinks (fst (ltl_step drinks (So
     apply simp
     apply (case_tac "aa = STR ''init'' \<and> ba = []")
    apply (simp add: possible_steps_init init_def)
-  apply (metis (no_types, lifting) make_full_observation.simps(1) option.inject state.ext_inject stream.sel(1) zero_neq_one)
+  apply (metis (no_types, lifting) make_full_observation.simps(1) option.inject state.ext_inject zero_neq_one)
   apply (simp add: possible_steps_not_init)
-  by (metis make_full_observation.simps(1) option.simps(3) state.ext_inject stream.sel(1))
+  by (metis make_full_observation.simps(1) option.simps(3) state.ext_inject)
 
 lemma state_none: "((StateEq None) impl nxt (StateEq None)) (make_full_observation e s r t)"
   by (simp add: StateEq_def)
@@ -96,17 +93,6 @@ lemma StateEq_alt: "alw (StateEq s) s' = alw (\<lambda>x. shd x = s) (smap (\<la
 lemma test: "statename (shd (make_full_observation e None r t)) = None"
   by simp
 
-lemma "alw (nxt (StateEq (Some 2)) impl (LabelEq ''vend'')) (watch drinks t)"
-proof(coinduction)
-  case alw
-  then show ?case
-    apply (case_tac "shd t")
-    apply (case_tac "a = STR ''init'' \<and> b = []")
-     defer
-     apply (simp add: possible_steps_not_init)
-    oops
-
-
 lemma "alw (\<lambda>s. StateEq None (stl s)) (make_full_observation drinks None Map.empty t)"
   by (metis alw_iff_sdrop once_none_always_none sdrop_simps(2))
 
@@ -127,10 +113,6 @@ lemma step_not_init: "t \<noteq> (STR ''init'', []) \<Longrightarrow> ltl_step d
   using no_possible_steps_not_init no_possible_steps
   by simp
 
-lemma updates_init: "apply_updates (Updates init) (case_vname Map.empty Map.empty) Map.empty = <R 1 := Num 0>"
-  apply (rule ext)
-  by (simp add: init_def)
-
 lemma ltl_step_alt [simp]:  "ltl_step e (Some s) r t = (let possibilities = possible_steps e s r (fst t) (snd t) in
                    if possibilities = {||} then (None, [], r)
                    else
@@ -145,30 +127,22 @@ lemma possible_steps_coin: "possible_steps drinks 1 r STR ''coin'' [] = {|(1, co
   apply safe
   by (simp_all add: vend_def coin_def)
 
-lemma possible_steps_vend_insufficient: "n \<le> 0 \<Longrightarrow> possible_steps drinks 1 <R 1 := Num n> STR ''vend'' [] = {||}"
+lemma possible_steps_vend_insufficient: "n \<le> 0 \<Longrightarrow> possible_steps drinks 1 <1 := Num n> STR ''vend'' [] = {||}"
   apply (simp add: possible_steps_def ffilter_def fset_both_sides Abs_fset_inverse Set.filter_def drinks_def)
   apply safe
-  by (simp_all add: vend_def coin_def gval.simps ValueGt_def)
+  by (simp_all add: vend_def coin_def apply_guards)
 
-lemma possible_steps_vend_sufficient: "n > 0 \<Longrightarrow> possible_steps drinks 1 <R 1 := Num n> STR ''vend'' [] = {|(2, vend)|}"
+lemma possible_steps_vend_sufficient: "n > 0 \<Longrightarrow> possible_steps drinks 1 <1 := Num n> STR ''vend'' [] = {|(2, vend)|}"
   apply (simp add: possible_steps_alt ffilter_def fset_both_sides Abs_fset_inverse Set.filter_def drinks_def)
   apply safe
-  by (simp_all add: vend_def coin_def gval.simps ValueGt_def)
+  by (simp_all add: vend_def coin_def apply_guards)
 
 lemma invalid_possible_steps_1: "shd t \<noteq> (STR ''coin'', []) \<Longrightarrow>
     shd t \<noteq> (STR ''vend'', []) \<Longrightarrow> possible_steps drinks 1 r (fst (shd t)) (snd (shd t)) = {||}"
   apply (simp add: possible_steps_def ffilter_def fset_both_sides Abs_fset_inverse drinks_def Set.filter_def)
   by (metis coin_def length_0_conv prod.collapse transition.ext_inject transition.surjective vend_def)
 
-lemma updates_coin: "(apply_updates (Updates coin) (case_vname Map.empty (\<lambda>na. if na = 1 then Some (Num n) else None)) <R 1 := Num n>) = <R 1 := Num (n + 1)>"
-  apply (rule ext)
-  by (simp add: coin_def)
-
-lemma updates_vend: "(apply_updates (Updates vend) (case_vname Map.empty (\<lambda>na. if na = 1 then Some (Num n) else None)) <R 1 := Num n>) = <R 1 := Num (n - 1)>"
-  apply (rule ext)
-  by (simp add: vend_def)
-
-lemma less_than_zero_not_nxt_2: "n \<le> 0 \<Longrightarrow> \<not>statename (shd (stl (make_full_observation drinks (Some 1) <R 1 := Num n> t))) = Some 2"
+lemma less_than_zero_not_nxt_2: "n \<le> 0 \<Longrightarrow> \<not>statename (shd (stl (make_full_observation drinks (Some 1) <1 := Num n> t))) = Some 2"
   apply (case_tac "shd t = (STR ''coin'', [])")
       apply (simp add: possible_steps_coin)
   apply (case_tac "shd t = (STR ''vend'', [])")
@@ -177,70 +151,6 @@ lemma less_than_zero_not_nxt_2: "n \<le> 0 \<Longrightarrow> \<not>statename (sh
 
 lemma possible_steps_2: "possible_steps drinks 2 r (fst (shd t)) (snd (shd t)) = {||}"
   by (simp add: possible_steps_def ffilter_def fset_both_sides Abs_fset_inverse Set.filter_def drinks_def)
-
-lemma stop_at_2_old: "alw (\<lambda>xs. statename (shd (stl xs)) = Some 2 \<longrightarrow> MaybeBoolInt (\<lambda>x y. y < x) (datastate (shd xs) (R 1)) (Some (Num 0)) = trilean.true)
-     (make_full_observation drinks (Some 2) <R 1 := Num (n - 1)> t)"
-proof(coinduction)
-  case alw
-  then show ?case
-    apply (simp add: possible_steps_2)
-    using once_none_always_none
-    by (simp add: StateEq_def alw_iff_sdrop)
-qed
-
-lemma reg_simp: "(\<lambda>a. if a = R 1 then Some (Num n) else None) = <R 1 := Num n>"
-  by (rule ext, simp)
-
-lemma once_none_no_change_data: "alw (\<lambda>xs. (datastate (shd xs)) = r) (make_full_observation e None r t)"
-proof(coinduction)
-  case alw
-  then show ?case
-    apply simp
-    by (simp add: all_imp_alw alw_inv)
-qed
-
-lemma shd_not_lt_zero: "0 \<le> n \<Longrightarrow> (\<lambda>xs. MaybeBoolInt (<) (datastate (shd xs) (R 1)) (Some (Num 0)) \<noteq> trilean.true) (make_full_observation drinks None <R 1 := Num n> t)"
-  by simp
-
-lemma nxt_not_lt_zero: "0 \<le> n \<Longrightarrow> nxt (\<lambda>xs. MaybeBoolInt (<) (datastate (shd xs) (R 1)) (Some (Num 0)) \<noteq> trilean.true) (make_full_observation drinks None <R 1 := Num n> t)"
-  by simp
-
-lemma once_none_remains_not_lt_zero: "0 \<le> n \<Longrightarrow> alw (\<lambda>xs. MaybeBoolInt (<) (datastate (shd xs) (R 1)) (Some (Num 0)) \<noteq> trilean.true) (make_full_observation drinks None <R 1 := Num n> t)"
-  using once_none_no_change_data
-  by (simp add: alw_iff_sdrop)
-
-lemma once_none_null_remains_not_lt_zero: "alw (\<lambda>xs. MaybeBoolInt (<) (datastate (shd xs) (R 1)) (Some (Num 0)) \<noteq> trilean.true) (make_full_observation drinks None Map.empty t)"
-  using once_none_no_change_data
-  by (simp add: alw_iff_sdrop)
-
-lemma stop_at_2: "0 \<le> n \<Longrightarrow>
-      alw (\<lambda>xs. MaybeBoolInt (<) (datastate (shd xs) (R 1)) (Some (Num 0)) \<noteq> trilean.true) (make_full_observation drinks (Some 2) <R 1 := Num n> t)"
-proof(coinduction)
-  case alw
-  then show ?case
-    by (simp add: possible_steps_2 once_none_remains_not_lt_zero)
-qed
-
-lemma next_not_lt_zero: "n \<ge> 0 \<Longrightarrow> nxt (\<lambda>xs. MaybeBoolInt (<) (datastate (shd xs) (R 1)) (Some (Num 0)) \<noteq> trilean.true) (make_full_observation drinks (Some 1) <R 1 := Num n> t)"
-    apply simp
-    apply (case_tac "shd t = (STR ''vend'', [])")
-    apply (case_tac "n = 0")
-      apply (simp add: possible_steps_vend_insufficient)
-     apply (simp add: possible_steps_vend_sufficient updates_vend)
-    apply (case_tac "shd t = (STR ''coin'', [])")
-    defer
-     apply (simp add: invalid_possible_steps_1)
-  by (simp add: possible_steps_coin updates_coin)
-
-lemma StateEq_None_not_Some: "StateEq None s \<Longrightarrow> \<not> StateEq (Some n) s"
-  by (simp add: StateEq_def)
-
-lemma not_initialised: "alw (\<lambda>xs. StateEq (Some 1) xs \<and>
-              MaybeBoolInt (<) (datastate (shd xs) (R 1)) (Some (Num 0)) = trilean.true \<and> LabelEq ''vend'' xs \<and> InputEq [] xs \<longrightarrow>
-              StateEq (Some 2) (stl xs))
-     (make_full_observation drinks None Map.empty t)"
-  using once_none_always_none StateEq_None_not_Some
-  by (simp add: alw_iff_sdrop)
 
 lemma implode_init: "String.implode ''init'' = STR ''init''"
   by (metis Literal.rep_eq String.implode_explode_eq zero_literal.rep_eq)
@@ -277,11 +187,15 @@ lemma possible_steps_0: "possible_steps drinks 0 Map.empty l i = finsert x S' \<
   using possible_steps_not_init
   by auto
 
-lemma vend_insufficient: "possible_steps drinks 1 <R 1 := Num 0> STR ''vend'' i = {||}"
+lemma apply_updates_init: "apply_updates (Updates init) <> <> = <1 := Num 0>"
+  apply (rule ext)
+  by (simp add: init_def)
+
+lemma vend_insufficient: "possible_steps drinks 1 <1 := Num 0> STR ''vend'' i = {||}"
   apply (simp add: possible_steps_def ffilter_def fset_both_sides Abs_fset_inverse Set.filter_def drinks_def)
   apply safe
    apply (simp add: coin_def)
-  by (simp add: vend_def gval.simps ValueGt_def)
+  by (simp add: vend_def apply_guards)
 
 lemma LTL_aux2: "((nxt (LabelEq ''vend'')) impl not (ev (StateEq (Some 2)))) (watch drinks t)"
   apply (simp add: watch_def LabelEq_def implode_vend not_ev_iff)
@@ -294,12 +208,12 @@ proof(coinduction)
      defer
     using possible_steps_not_init alw_not_some
      apply (simp add: no_possible_steps_not_init)
-    apply (simp add: possible_steps_init updates_init)
+    apply (simp add: possible_steps_init apply_updates_init)
     apply (rule disjI2)
   proof(coinduction)
     case alw
     then show ?case
-      apply (simp add: vend_insufficient)
+      apply (simp add: vend_insufficient apply_updates_init)
       apply (rule disjI2)
       using alw_not_some
       by simp
@@ -308,13 +222,10 @@ qed
 
 lemma LTL_init_makes_r_1_zero: "((LabelEq ''init'' aand InputEq []) impl nxt (checkInx rg 1 ValueEq (Some (Num 0)))) (watch drinks t)"
   apply (case_tac "shd t = (STR ''init'', [])")
-   apply (simp add: possible_steps_init updates_init ValueEq_def watch_def)
+   apply (simp add: possible_steps_init apply_updates_init ValueEq_def watch_def)
   apply clarify
   using not_init
   by simp
-
-lemma LTL_must_pay_wrong: "((not (LabelEq ''vend'' suntil LabelEq ''coin'')) suntil StateEq None) (watch drinks t)"
-  oops
 
 lemma shd_not_init: "shd t \<noteq> (STR ''init'', []) \<Longrightarrow> \<not> ev (\<lambda>s. statename (shd s) = Some 2) (make_full_observation drinks (Some 0) Map.empty t)"
   apply (simp add: not_ev_iff)
@@ -327,7 +238,7 @@ proof(coinduction)
     by (simp add: possible_steps_not_init alw_not_some)
 qed
 
-lemma vend_gets_stuck: "stl t = (STR ''vend'', []) ## x2 \<Longrightarrow> \<not>ev (\<lambda>s. statename (shd s) = Some 2) (make_full_observation drinks (Some 1) <R 1 := Num 0> ((STR ''vend'', []) ## x2))"
+lemma vend_gets_stuck: "stl t = (STR ''vend'', []) ## x2 \<Longrightarrow> \<not>ev (\<lambda>s. statename (shd s) = Some 2) (make_full_observation drinks (Some 1) <1 := Num 0> ((STR ''vend'', []) ## x2))"
   apply (simp add: not_ev_iff)
 proof(coinduction)
   case alw
@@ -337,17 +248,16 @@ qed
 
 lemma possible_steps_1_invalid: "x1 \<noteq> (STR ''coin'', []) \<Longrightarrow>
        x1 \<noteq> (STR ''vend'', []) \<Longrightarrow>
-       possible_steps drinks 1 <R 1 := Num 0> (fst x1) (snd x1) = {||}"
+       possible_steps drinks 1 <1 := Num 0> (fst x1) (snd x1) = {||}"
   apply (simp add: possible_steps_def ffilter_def fset_both_sides Abs_fset_inverse drinks_def Set.filter_def)
   apply safe
    apply (simp add: coin_def)
    apply (metis prod.collapse)
-  by (simp add: vend_def gval.simps ValueGt_def)
-
+  by (simp add: vend_def apply_guards)
 
 lemma invalid_gets_stuck: "x1 \<noteq> (STR ''coin'', []) \<Longrightarrow>
                            x1 \<noteq> (STR ''vend'', []) \<Longrightarrow>
-                           \<not>ev (\<lambda>s. statename (shd s) = Some 2) (make_full_observation drinks (Some 1) <R 1 := Num 0> (x1 ## x2))"
+                           \<not>ev (\<lambda>s. statename (shd s) = Some 2) (make_full_observation drinks (Some 1) <1 := Num 0> (x1 ## x2))"
   apply (simp add: not_ev_iff)
 proof(coinduction)
   case alw
@@ -366,7 +276,7 @@ proof(coinduction)
      defer
     apply (simp add: decompose_pair)
      apply (simp add: possible_steps_not_init alw_not_some)
-    apply (simp add: possible_steps_init updates_init)
+    apply (simp add: possible_steps_init apply_updates_init)
     apply (rule disjI2)
   proof(coinduction)
     case alw
@@ -392,12 +302,11 @@ proof(coinduction)
      apply (simp only: decompose_pair)
     using possible_steps_not_init alw_not_some
      apply simp
-    apply (simp add: possible_steps_init updates_init)
+    apply (simp add: possible_steps_init apply_updates_init)
     apply (rule disjI2)
     using invalid_gets_stuck[of "shd (stl t)" "stl (stl t)"]
     by (simp add: alw_ev)
 qed
-
 
 (* Ramsay, this is the proof you want!
    I'll convert it to an Isabelle code snippet for the actual paper to make it really pretty but for
@@ -411,7 +320,7 @@ lemma LTL_must_pay_correct: "((ev (StateEq (Some 2))) impl (not(LabelEq ''vend''
    apply (simp add: shd_not_init)
   apply (rule suntil.step)
    apply simp
-  apply (simp add: possible_steps_init updates_init)
+  apply (simp add: possible_steps_init apply_updates_init)
   apply (case_tac "shd (stl t) = (STR ''coin'', [])")
    apply (simp add: suntil.base)
   apply (case_tac "shd (stl t) = (STR ''vend'', [])")
