theories/SAL-examples/Drinks_Machine_Change.thy
@@ -1,5 +1,5 @@
 theory Drinks_Machine_Change
-  imports "../examples/Drinks_Machine"
+  imports Drinks_Machine
 begin
 
 definition vend :: "transition" where
@@ -8,7 +8,7 @@ definition vend :: "transition" where
         Arity = 0,
         Guard = [(Ge (V (R 2)) (L (Num 100)))], \<comment>\<open> This is syntactic sugar for ''Not (Lt (V (R 2)) (N 100))'' which could also appear \<close>
         Outputs =  [(V (R 1)), (Minus (V (R 2)) (L (Num 100)))],
-        Updates = [(R 1, (V (R 1))), (R 2, (V (R 2)))]
+        Updates = [(1, (V (R 1))), (2, (V (R 2)))]
       \<rparr>"
 
 definition drinks :: transition_matrix where
@@ -19,9 +19,6 @@ definition drinks :: transition_matrix where
          |}"
 
 lemmas transitions = select_def coin_def vend_def
-
-lemma "observe_trace drinks 0 <> [] = []"
-  by (simp add: observe_trace_def)
 
 lemma possible_steps_0:  "length i = 1 \<Longrightarrow> possible_steps drinks 0 Map.empty ((STR ''select'')) i = {|(1, select)|}"
   apply (simp add: possible_steps_def drinks_def transitions)
@@ -36,38 +33,54 @@ lemma possible_steps_1_coin: "possible_steps drinks 1 r (STR ''coin'') [Num n'] 
   apply (simp add: possible_steps_def drinks_def transitions)
   by force
 
-lemma possible_steps_1_vend: "n \<ge> 100 \<Longrightarrow> possible_steps drinks 1 <R 1 := Str ''coke'', R 2 := Num n> (STR ''vend'') [] = {|(2, vend)|}"
-proof-
-  assume premise: "n \<ge> 100"
-  have filter: " ffilter
-     (\<lambda>((origin, dest), t).
-         origin = 1 \<and>
-         Label t = STR ''vend'' \<and>
-         Arity t = 0 \<and>
-         apply_guards (Guard t) (\<lambda>x. case x of I n \<Rightarrow> input2state [] 1 (I n) | R na \<Rightarrow> <R 1 := EFSM.Str ''coke'', R 2 := Num n> (R na)))
-     Drinks_Machine_Change.drinks =
-    {|((1, 2), Drinks_Machine_Change.vend)|}"
-    using premise
-    apply (simp add: ffilter_def drinks_def fset_both_sides Abs_fset_inverse Set.filter_def)
-    apply safe
-    by (simp_all add: transitions gval.simps ValueGt_def)
-  show ?thesis
-    by (simp add: possible_steps_def filter)
-qed
+lemma possible_steps_1_vend: "r 2 = Some (Num n) \<and> n \<ge> 100 \<Longrightarrow> possible_steps drinks 1 r (STR ''vend'') [] = {|(2, vend)|}"
+  apply (simp add: possible_steps_singleton drinks_def)
+  apply safe
+  by (simp_all add: transitions apply_guards)
 
 lemma "observe_trace drinks 0 <> [((STR ''select''), [Str ''coke'']), ((STR ''coin''), [Num 50]), ((STR ''coin''), [Num 50]), ((STR ''vend''), [])] = [[], [Some (Num 50)], [Some (Num 100)], [Some (Str ''coke''), Some (Num 0)]]"
-  unfolding observe_trace_def observe_all_def step_def
-  apply (simp add: possible_steps_0 updates_select outputs_select)
-  apply (simp add: possible_steps_1_coin updates_coin)
-  apply (simp add: possible_steps_1_vend)
-  by (simp add: coin_def vend_def)
+  apply (rule observe_trace_possible_step)
+     apply (simp add: possible_steps_0)
+    apply (simp add: select_def)
+   apply simp
+  apply (rule observe_trace_possible_step)
+     apply (simp add: possible_steps_1_coin)
+    apply (simp add: coin_def apply_outputs select_def)
+   apply simp
+  apply (rule observe_trace_possible_step)
+     apply (simp add: possible_steps_1_coin)
+    apply (simp add: coin_def apply_outputs select_def)
+   apply simp
+  apply (rule observe_trace_possible_step)
+     apply simp
+     apply (rule possible_steps_1_vend)
+     apply (simp add: coin_def select_def datastate)
+     apply auto[1]
+    apply (simp add: vend_def apply_outputs coin_def select_def)
+   apply simp
+  by simp
 
 lemma "observe_trace drinks 0 <> [((STR ''select''), [Str ''coke'']), ((STR ''coin''), [Num 50]), ((STR ''coin''), [Num 100]), ((STR ''vend''), [])] = [[], [Some (Num 50)], [Some (Num 150)], [Some (Str ''coke''), Some (Num 50)]]"
-  unfolding observe_trace_def observe_all_def step_def
-  apply (simp add: possible_steps_0 updates_select outputs_select)
-  apply (simp add: possible_steps_1_coin updates_coin)
-  apply (simp add: possible_steps_1_vend)
-  by (simp add: coin_def vend_def)
+  apply (rule observe_trace_possible_step)
+     apply (simp add: possible_steps_0)
+    apply (simp add: select_def)
+   apply simp
+  apply (rule observe_trace_possible_step)
+     apply (simp add: possible_steps_1_coin)
+    apply (simp add: coin_def apply_outputs select_def)
+   apply simp
+  apply (rule observe_trace_possible_step)
+     apply (simp add: possible_steps_1_coin)
+    apply (simp add: coin_def apply_outputs select_def)
+   apply simp
+  apply (rule observe_trace_possible_step)
+     apply simp
+     apply (rule possible_steps_1_vend)
+     apply (simp add: coin_def select_def datastate)
+     apply auto[1]
+    apply (simp add: vend_def apply_outputs coin_def select_def)
+   apply simp
+  by simp
 
 lemma possible_steps_invalid: "l \<noteq> (STR ''coin'') \<and> l \<noteq> (STR ''vend'') \<Longrightarrow> possible_steps drinks 1 d l i = {||}"
   apply (simp add: possible_steps_def drinks_def transitions)
@@ -75,8 +88,11 @@ lemma possible_steps_invalid: "l \<noteq> (STR ''coin'') \<and> l \<noteq> (STR 
 
 (* Stop when we hit a spurious input *)
 lemma "observe_trace drinks 0 <> [((STR ''select''), [Str ''coke'']), ((STR ''invalid''), [Num 50])] = [[]]"
-  unfolding observe_trace_def observe_all_def step_def
-  apply (simp add: possible_steps_0 updates_select outputs_select)
+  apply (rule observe_trace_possible_step)
+     apply (simp add: possible_steps_0)
+    apply (simp add: select_def)
+   apply simp
+  apply (rule observe_trace_no_possible_step)
   by (simp add: possible_steps_invalid)
 
 lemma invalid_input: "\<not> accepts drinks 1 d' [((STR ''invalid''), [Num 50])]"
@@ -89,7 +105,6 @@ lemma invalid_input: "\<not> accepts drinks 1 d' [((STR ''invalid''), [Num 50])]
   by auto
 
 lemma invalid_valid_prefix: "\<not> (accepts_trace (drinks) [((STR ''select''), [Str ''coke'']), ((STR ''invalid''), [Num 50])])"
-  unfolding accepts_trace_def
   apply clarify
   apply (rule EFSM.accepts.induct)
     apply simp
@@ -101,12 +116,15 @@ lemma invalid_valid_prefix: "\<not> (accepts_trace (drinks) [((STR ''select''), 
    apply simp
   apply (simp add: step_def)
   apply clarify
-  apply (simp add: possible_steps_0 outputs_select updates_select)
+  apply (simp add: possible_steps_0 outputs_select)
   using invalid_input
   by simp
 
 lemma "observe_trace drinks 0 <> [((STR ''select''), [Str ''coke'']), ((STR ''invalid''), [Num 50]), ((STR ''coin''), [Num 50])] = [[]]"
-  unfolding observe_trace_def observe_all_def step_def
-  apply (simp add: possible_steps_0 outputs_select updates_select)
+  apply (rule observe_trace_possible_step)
+     apply (simp add: possible_steps_0)
+    apply (simp add: select_def)
+   apply simp
+  apply (rule observe_trace_no_possible_step)
   by (simp add: possible_steps_invalid)
 end
