theories/SAL-examples/Inference_Answer.thy
@@ -2,10 +2,10 @@ theory Inference_Answer
   imports "../EFSM"
 begin
 definition select :: transition where
-  "select = \<lparr>Label = STR ''select'', Arity = 1, Guard = [], Outputs = [], Updates = [(R 2, L (Num 0)), (R 1, V (I 1))]\<rparr>"
+  "select = \<lparr>Label = STR ''select'', Arity = 1, Guard = [], Outputs = [], Updates = [(2, L (Num 0)), (1, V (I 1))]\<rparr>"
 
 definition coin :: transition where
-  "coin = \<lparr>Label = STR ''coin'', Arity = 1, Guard = [], Outputs = [Plus (V (R 2)) (V (I 1))], Updates = [(R 2, Plus (V (R 2)) (V (I 1)))]\<rparr>"
+  "coin = \<lparr>Label = STR ''coin'', Arity = 1, Guard = [], Outputs = [Plus (V (R 2)) (V (I 1))], Updates = [(2, Plus (V (R 2)) (V (I 1)))]\<rparr>"
 
 definition vend :: transition where
   "vend = \<lparr>Label = STR ''vend'', Arity = 0, Guard = [], Outputs = [V (R 1)], Updates = []\<rparr>"
